src/HOL/Word/Bits.thy
@@ -25,12 +25,10 @@ text \<open>Testing and shifting operations.\<close>
 class bits = bit +
   fixes test_bit :: "'a \<Rightarrow> nat \<Rightarrow> bool"  (infixl "!!" 100)
     and lsb :: "'a \<Rightarrow> bool"
+    and msb :: "'a \<Rightarrow> bool"
     and set_bit :: "'a \<Rightarrow> nat \<Rightarrow> bool \<Rightarrow> 'a"
     and set_bits :: "(nat \<Rightarrow> bool) \<Rightarrow> 'a"  (binder "BITS " 10)
     and shiftl :: "'a \<Rightarrow> nat \<Rightarrow> 'a"  (infixl "<<" 55)
     and shiftr :: "'a \<Rightarrow> nat \<Rightarrow> 'a"  (infixl ">>" 55)
-
-class bitss = bits +
-  fixes msb :: "'a \<Rightarrow> bool"
 
 end
